wip

Judge.v
@@ -15,12 +15,12 @@ Reserved Notation "( Φ ; Γ ; S ; Ξ ) ⊢ s ::: ( O ; H )"
 
 Definition wf_subst θ := forall v, θ v = ν <-> v = ν.
 
-(* Inductive wf_type : type_env -> heap_env -> reft_type -> Prop := *)
-(* | wf_reft_t : forall Γ Σ b p, wf_prop Γ Σ p -> *)
-(* (* ------------------------------------------------------------------- *) *)
-(*   wf_type Γ Σ { ν : b | p } *)
+Inductive wf_type : type_env -> heap_env -> reft_type -> Prop :=
+| wf_reft_t : forall Γ Σ b p, wf_prop Γ Σ p ->
+(* ------------------------------------------------------------------- *)
+  wf_type Γ Σ { ν : b | p }
 
-Inductive wf_prop : type_env -> heap_env -> reft_prop -> Prop :=
+with wf_prop : type_env -> heap_env -> reft_prop -> Prop :=
 | wf_tt : forall Γ Σ, 
 (* ------------------------------------------------------------------- *)
             wf_prop Γ Σ tt_r 
@@ -41,8 +41,7 @@ Inductive wf_prop : type_env -> heap_env -> reft_prop -> Prop :=
 (* ------------------------------------------------------------------- *)
   wf_prop Γ Σ (or_r p1 p2)
 
-with 
-wf_expr : type_env -> heap_env -> expr -> Prop :=
+with  wf_expr : type_env -> heap_env -> expr -> Prop :=
 | wf_val : forall Γ Σ v,
 (* ------------------------------------------------------------------- *)
   wf_expr Γ Σ (value_e v)
@@ -64,15 +63,8 @@ wf_expr : type_env -> heap_env -> expr -> Prop :=
 (* ------------------------------------------------------------------- *)
   wf_expr Γ Σ (fun_e f e1 e2).
 
-Definition wf_type Γ Σ (T : reft_type) := 
-  let (b, p) := T in
-  match b with
-    | ref_t v => bind_not_in v Σ /\ wf_prop Γ Σ p
-    | _       => wf_prop Γ Σ p
-  end.
-
-Definition fresh x Γ Σ :=
-  x <> ν /\ var_not_in x Γ /\ loc_not_in x Σ /\ bind_not_in x Σ.
+Definition fresh x Γ Σ := x <> ν /\ var_not_in x Γ /\ bind_not_in x Σ.
+Definition fresh_loc l Γ Σ := loc_not_in l Σ /\ loc_not_in_ctx l Γ.
             
 Inductive wf_env : heap_env -> type_env -> Prop :=
   | wf_env_nil : forall Σ,
@@ -93,7 +85,7 @@ Inductive wf_heap : type_env -> heap_env -> heap_env -> Prop :=
 
   | wf_heap_bind :
       forall Γ Σ Σ0 l x t,
-        fresh x Γ Σ0 -> fresh l Γ Σ0 -> l <> x -> 
+        fresh x Γ Σ0 -> fresh_loc l Γ Σ0 -> bind_in x Σ ->
         wf_type Γ Σ t -> wf_heap Γ Σ Σ0 ->
 (* ------------------------------------------------------------------- *)
     wf_heap Γ Σ ((l, (x, t)) :: Σ0).
@@ -190,8 +182,8 @@ Definition join_heap Γ1 Γ2 Γ Ξ Σ1 Σ2 Σ :=
     /\ heap_subtype Γ1 Ξ Σ1 Σ 
     /\ heap_subtype Γ2 Ξ Σ2 Σ.
 
-Definition isub {A D R : Type} {S : Subst A D R }
-                (θ : subst_t D R) (θl : subst_t D R) (t : A) 
+Definition isub {A D R : Type} {S : Subst A D R } {SL : Subst A loc loc}
+                (θ : subst_t D R) (θl : subst_t loc loc) (t : A) 
   := subst θl (subst θ t).
                               
 Inductive stmt_type : proc_env -> 
@@ -208,7 +200,7 @@ Inductive stmt_type : proc_env ->
    (Φ ; Γ ; Σ ; Ξ) ⊢ skip_s ::: (Γ ; Σ)
 
 | t_proc_s :
-    forall Φ Γ Σ Σu Σm Ξ (v:var) f p S (θ : var -> var) (θl : var -> var),
+    forall Φ Γ Σ Σu Σm Ξ (v:var) f p S (θ : var -> var) (θl : loc -> loc),
       (f,(p,S)) ∈ Φ -> wf_schema S -> wf_subst θ -> heap_split Σu Σm Σ ->
       (forall x, θ x = (subst θ (fst (s_ret S))) <-> x = (fst (s_ret S))) ->
       (forall x', ~(In x' (fst (s_ret S) :: s_formals S)) -> θ x' = x') ->
@@ -225,7 +217,7 @@ Inductive stmt_type : proc_env ->
 
 | t_pad : 
     forall Φ Γ Σ Ξ l x a t,
-      fresh x Γ Σ -> fresh a Γ Σ -> fresh l Γ Σ -> wf_type Γ Σ t ->
+      fresh x Γ Σ -> fresh a Γ Σ -> fresh_loc l Γ Σ -> wf_type Γ Σ t ->
 (* ------------------------------------------------------------------- *)
       ((Φ ; Γ ; Σ ; Ξ) ⊢ pad_s a x ::: (Γ ; (l,(x,t))::Σ))
 
